use the bn_mul_by_limb_add_shift_j function in montgomery_reduction

code/experimental/rsapss/Hacl.Spec.Bignum.Montgomery.fst
@@ -28,9 +28,7 @@ val mont_reduction_:
 
 let mont_reduction_ #nLen #rLen n nInv_u64 j res =
   let qj = nInv_u64 *. res.[j] in
-  let res' = sub res j nLen in
-  let c, res' = bn_mul_by_limb_add #nLen n qj res' in
-  let res = update_sub res j nLen res' in
+  let c, res' = bn_mul_by_limb_add_shift_j #nLen #(rLen + rLen) n qj j res in
 
   let res' = sub res (j + nLen) (rLen + rLen - j - nLen) in
   let _, res' = bn_add res' (create 1 c) in
